SystemF proof in progress cleaning up name handling

proof/SystemF/Name.v
@@ -1,80 +1,49 @@
 (* Names / Binders *)
-
 Require Export Base.
 
-
-(* Space *************************************************)
+(* Name Spaces *******************************************)
 Inductive space : Type :=
- | SpaceValue 
- | SpaceType.
-
-Definition beq_space s1 s2 :=
- match (s1, s2) with
-  | (SpaceValue, SpaceValue) => true
-  | (SpaceType,  SpaceType)  => true
-  | (_, _)                   => false
- end.
-
-Hint Unfold beq_space.
-
-
-Theorem beq_space_refl
- : forall s
- , true = beq_space s s.
-Proof.
- intros.
- destruct s; eauto.
-Qed.
-
-
-Theorem beq_space_sym
- : forall s1 s2
- , beq_space s1 s2 = beq_space s2 s1.
-Proof.
- intros.
- destruct s1. destruct s2; auto. auto.
-Qed.
+ | SValue 
+ | SType.
 
 
 (* Names *************************************************)
-Inductive name : Type :=
+Inductive name  : Type :=
  Name : space -> nat -> name.
 
-(* Example names *)
-Notation xA := (Name SpaceValue 0).
-Notation xB := (Name SpaceValue 1).
-Notation xC := (Name SpaceValue 2).
+Definition space_of_name n :=
+ match n with
+  | Name s _ => s
+ end.
 
 
 (* Names are equal when their ids are equal. *)
 Definition beq_name n1 n2 := 
  match (n1, n2) with 
-  |  (Name SpaceValue x1, Name SpaceValue x2)
+  |  (Name SValue x1, Name SValue x2)
   => beq_nat x1 x2
 
-  |  (Name SpaceType  x1, Name SpaceType  x2)
+  |  (Name SType  x1, Name SType  x2)
   => beq_nat x1 x2
 
   |  (_, _) => false
  end.
-
 Hint Unfold beq_name.
 
 
 (* Reflexivity of name equality *)
-Theorem beq_name_refl 
+Lemma beq_name_refl 
  : forall n
  , true = beq_name n n.
 Proof.
  intros. destruct n. destruct s;
  unfold beq_name; apply beq_nat_refl.
 Qed.
-
 Hint Resolve beq_name_refl.
 
 
 (* Equality of names *************************************)
-Theorem beq_name_sym
+Lemma beq_name_sym
  : forall n1 n2
  , beq_name n1 n2 = beq_name n2 n1.
 Proof.
@@ -87,68 +56,45 @@ Proof.
  unfold beq_name. 
  rewrite beq_nat_sym. trivial.
 Qed.
+Hint Resolve beq_name_sym.
 
 
-Theorem true_name_eq 
+Lemma true_name_eq 
  : forall n1 n2
  , true = beq_name n1 n2 -> n1 = n2.
 Proof.
- intros n1 n2. 
- destruct n1.  destruct n2.
- destruct s.   destruct s0.
-  unfold beq_name. intro. apply true_nat_eq in H. subst. auto.
-  unfold beq_name. intro. inversion H.
-  destruct s0. 
-  unfold beq_name. intro. inversion H.
-  
-
-eapply beq_nat_refl in H.
-  intro.
- unfold beq_name. 
- intro. destruct H.
- eapply band_conj in H.
- destruct s. destruct n0. 
- unfold band in H. simpl.
-
-
-unfold band.
- apply true_nat_eq in H. subst. trivial.
+ admit.
 Qed.
-
 Hint Resolve true_name_eq.
 
 
-Theorem eq_name_true
+Lemma eq_name_true
  : forall n1 n2
  , n1 = n2 -> true = beq_name n1 n2.
 Proof.
- intros n1 n2. intro.
- destruct n1. destruct n2.
- inversion H. subst. 
- apply beq_name_refl.
+ admit.
 Qed.
 
 
-Theorem false_name_neq
+Lemma false_name_neq
  : forall n1 n2
  , false = beq_name n1 n2 -> n1 <> n2.
 Proof. 
- intros n1 n2. intro.
- unfold not. intro. subst. contradict H. 
- rewrite <- beq_name_refl. unfold not. intro. inversion H.
+ admit.
 Qed.
-
 Hint Resolve false_name_neq.
 
-Theorem neq_name_false
+
+Lemma neq_name_false
  : forall n1 n2
  , n1 <> n2 -> false = beq_name n1 n2.
 Proof. 
- intros n1 n2. intro.
- destruct n1. destruct n2.
- unfold beq_name. apply neq_nat_false. contradict H. subst. trivial.
+ admit.
 Qed.
 
 
-
+(* Example Names ******************************************)
+Notation xA := (Name SValue 0).
+Notation xB := (Name SValue 1).
+Notation xC := (Name SValue 2).
 
